cleanup in CRF

src/tls/Hashing.CRF.fst
@@ -21,45 +21,37 @@ module MR = FStar.Monotonic.RRef
 module MM = MonotoneMap
 
 // the precise types guarantee that the table stays empty when crf _ = false
-type range = | Computed: a: alg {crf a} -> tag a -> range
-type domain = fun (Computed a t) -> b:bytes { Seq.equal (hash a b) t }
+private type range = | Computed: a: alg {crf a} -> tag a -> range
+private type domain = fun (Computed a t) -> b:bytes { Seq.equal (hash a b) t }
 
-let inv (f:MM.map' range domain) = True 
-
-(* avoiding:
-  // when computed, f is injective on each collision-resistant algorithm
-  forall (a:alg{crf a}) (b0:bytes) (b1:bytes). 
-    ( match f (a,b0), f(a,b1) with 
-      | Some h0, Some h1 -> Seq.equal h0 h1 ==> Seq.equal b0 b1 
-      | _ -> True *)
-
-let table = MM.alloc #TLSConstants.tls_tables_region #range #domain #inv
-
+private let inv (f:MM.map' range domain) = True // a bit overkill? 
+private let table = MM.alloc #TLSConstants.tls_tables_region #range #domain #inv
 
 // witnessing that we hashed this particular content (for collision detection)
 // to be replaced by a witness of inclusion in a global table of all hash computations.
 // (not sure how to manage that table)
 
 //val hashed: a:alg -> b:bytes -> Type
-abstract type hashed a b = 
+abstract type hashed (a:alg) (b:bytes) = 
   crf a ==> (
     let h = hash a b in 
     let b: domain (Computed a h) = b in 
     MR.witnessed (MM.contains table (Computed a h) b))
 
 val crf_injective (a:alg) (b0:bytes) (b1:bytes): ST unit 
-  (requires (fun h0 -> hashed a b0 /\ hashed a b1 /\ Seq.equal (hash a b0) (hash a b1)))
-  (ensures (fun h0 _ h1 -> crf a ==> Seq.equal b0 b1))
+  (requires (fun h0 -> hashed a b0 /\ hashed a b1 ))
+  (ensures (fun h0 _ h1 -> crf a /\ hash a b0 =  hash a b1 ==> Seq.equal b0 b1))
 let crf_injective a b0 b1 =
   if crf a then (
     MR.m_recall table;
     let f = MR.m_read table in
-    let h = hash a b0 in 
-    MR.testify(MM.contains table (Computed a h) b0);
-    MR.testify(MM.contains table (Computed a h) b1);
+    let h0 = hash a b0 in 
+    let h1 = hash a b1 in 
+    MR.testify(MM.contains table (Computed a h0) b0);
+    MR.testify(MM.contains table (Computed a h1) b1);
   ())
 
-val stop: s:string -> ST 'a 
+private val stop: s:string -> ST 'a 
   (requires (fun h -> True))
   (ensures (fun h0 r h1 -> False))
 let rec stop (s:string) = stop s 
@@ -71,22 +63,39 @@ val finalize:
   ST (lbytes (tagLen a))
   (requires (fun h0 -> True))
   (ensures (fun h0 t h1 -> 
-    //TODO modifies table /\
     let b = content v in 
+    modifies (Set.singleton TLSConstants.tls_tables_region) h0 h1 /\ // precise enough? 
     t = hash a b /\ hashed a b 
   ))
 
 let finalize #a v = 
   let b = Hashing.content v in 
   let h = Hashing.finalize v in 
-  if crf a then 
+  if crf a then (
     let x = Computed a h in 
-    ( match MM.lookup table x with 
-      | None -> MM.extend table x b; h
-      | Some b' -> 
-          if b = b' then h 
-          else stop "hash collision detected" )
-  else h
+    match MM.lookup table x with 
+      | None -> MM.extend table x b
+      | Some b' -> if b <> b' then stop "hash collision detected");
+  h
 
 
+// sanity check
+private val test: a:alg -> b0:bytes -> b1:bytes -> unit 
+let test a b0 b1 = 
+  // we need to record *both* computations
+  let h = finalize (extend (start a) b0) in 
+  let h' = finalize (extend (extend (start a) b1) b1) in 
 
+  // ...and, annoyingly, to normalize concatenations
+  assert(Seq.equal (empty_bytes @| b0) b0);
+  assert(Seq.equal ((empty_bytes @| b1) @| b1) (b1 @| b1));
+
+  if h <> h' then assert(b0 <> b1 @| b1);
+
+  // ...and to apply a stateful lemma
+  crf_injective a b0 (b1 @| b1);
+  if h = h' then assert(crf a ==> b0 = b1 @| b1)
+  
+
+  
+  
